theories/RTac/Intro.v
@@ -109,8 +109,22 @@ Section parameterized.
       inv_all; subst.
       destruct Hopen as [ ? [ ? ? ] ].
       rewrite H3.
-      simpl. admit.
-    }
+      simpl. autorewrite with eq_rw.
+      eapply ctxD'_no_hyps; intros.
+      split; eauto.
+      eapply H6.
+      destruct H8. exists x1. destruct H8. revert H9. revert H5. clear.
+      generalize dependent (rev_involutive_trans (getUVars ctx nil)).
+      generalize dependent (rev_involutive_trans (getVars ctx nil)).
+      generalize dependent (getVars ctx nil).
+      generalize dependent (getUVars ctx nil).
+      intros.
+      generalize dependent (hlist_rev us).
+      generalize dependent (hlist_rev vs).
+      generalize dependent (rev t1).
+      generalize dependent (rev t0).
+      intros. destruct e0. destruct e.
+      rewrite H5. assumption. }
     { simpl. forward.
       eapply exprD'_typ0_weakenV with (tvs' := t :: nil) in H0; eauto.
       (** Same proof as above **)
@@ -126,149 +140,3 @@ Section parameterized.
   Qed.
 
 End parameterized.
-
-
-(*
-  Lemma _impls_sem
-  : forall ls P,
-      _impls ls P <-> (Forall (fun x => x) ls -> P).
-  Proof.
-    induction ls; simpl; intros.
-    + intuition.
-    + rewrite IHls. intuition.
-      inversion H0. eapply H; eauto.
-  Qed.
-  Lemma _exists_iff
-  : forall ls P Q,
-      (forall x, P x <-> Q x) ->
-      (@_exists ls P <-> @_exists ls Q).
-  Proof.
-    clear.
-    induction ls; simpl; intros.
-    + eapply H.
-    + apply exists_iff; intro. eapply IHls.
-      intro; eapply H.
-  Qed.
-  Lemma _forall_iff
-  : forall ls P Q,
-      (forall x, P x <-> Q x) ->
-      (@_foralls ls P <-> @_foralls ls Q).
-  Proof.
-    clear.
-    induction ls; simpl; intros.
-    + eapply H.
-    + apply forall_iff; intro. eapply IHls.
-      intro; eapply H.
-  Qed.
-
-  Lemma at_bottom_sound_option
-  : forall goal tus tvs f goal',
-      (forall tus' tvs' s e e',
-         f (tus ++ tus') (tvs ++ tvs') s e = Some e' ->
-         WellFormed_subst s ->
-         match goalD (tus ++ tus') (tvs ++ tvs') (GGoal s e)
-             , goalD (tus ++ tus') (tvs ++ tvs') e'
-         with
-           | None , _ => True
-           | Some _ , None => False
-           | Some g , Some g' =>
-             forall us vs,
-               g' us vs -> g us vs
-         end) ->
-      at_bottom f tus tvs goal = Some goal' ->
-      forall (Hwf : WellFormed_goal goal),
-      match goalD tus tvs goal
-          , goalD tus tvs goal'
-      with
-        | None , _ => True
-        | Some _ , None => False
-        | Some g , Some g' =>
-          forall us vs,
-            g' us vs -> g us vs
-      end.
-  Proof.
-    induction goal; simpl; intros.
-    { forwardy. inv_all; subst.
-      eapply IHgoal in H0; clear IHgoal; auto.
-      { simpl. forward. auto. }
-      { intros.
-        specialize (H tus' (t :: tvs') s e).
-        rewrite app_ass in H1. simpl in *.
-        eapply H in H1; clear H; auto.
-        forward.
-        rewrite substD_conv
-           with (pfu := eq_refl _) (pfv := eq_sym (HList.app_ass_trans _ _ _)) in H.
-        unfold propD in *.
-        rewrite exprD'_typ0_conv with (pfu := eq_refl _)
-             (pfv := eq_sym (HList.app_ass_trans _ _ _)) in H.
-        simpl in *.
-        unfold ResType in *.
-        autorewrite with eq_rw in *.
-        destruct e; forwardy.
-        { inv_all; subst.
-          rewrite H in *.
-          autorewrite with eq_rw in H3.
-          forwardy.
-          rewrite H3 in *.
-          inv_all; subst.
-          rewrite goalD_conv with (pfu := eq_refl)
-                                  (pfv := eq_sym (HList.app_ass_trans _ _ _)).
-          simpl.
-          forwardy.
-          autorewrite with eq_rw.
-          rewrite H1.
-          intros us vs. autorewrite with eq_rw.
-          clear - H4.
-          match goal with
-            | |- _ _ match ?X with _ => _ end ->
-                 _ _ match ?Y with _ => _ end /\
-                 _ _ match ?Z with _ => _ end =>
-              change X with Y ; change Z with Y ; destruct Y
-          end.
-          eauto. }
-        { rewrite H in *.
-          rewrite goalD_conv with (pfu := eq_refl)
-                                  (pfv := eq_sym (HList.app_ass_trans _ _ _)).
-          simpl.
-          forwardy.
-          autorewrite with eq_rw.
-          rewrite H1. intros.
-          inv_all; subst.
-          revert H6.
-          match goal with
-            | |- match ?X with _ => _ end _ _ ->
-                 match ?Y with _ => _ end _ _ =>
-              change Y with X ; destruct X
-          end. auto. } } }
-    { forwardy; inv_all; subst.
-      eapply IHgoal in H0; clear IHgoal; auto.
-      + simpl; forward; eauto.
-        destruct H3. eauto.
-      + intros.
-        rewrite goalD_conv
-           with (pfu := eq_sym (HList.app_ass_trans _ _ _))
-                (pfv := eq_refl).
-        autorewrite with eq_rw.
-        simpl. forward.
-        rewrite HList.app_ass_trans in H1.
-        simpl in H1.
-        eapply H in H1; clear H; eauto.
-        destruct e; forward.
-        - inv_all; subst.
-          revert H7. autorewrite with eq_rw.
-          eauto.
-        - inv_all; subst.
-          revert H6. autorewrite with eq_rw.
-          eauto. }
-    { forwardy; inv_all; subst.
-      eapply IHgoal in H0; clear IHgoal; eauto.
-      + simpl; forward; eauto.
-        inv_all. subst.
-        eapply _impls_sem; intro.
-        eapply _impls_sem in H5; eauto. }
-    { specialize (H nil nil s o goal').
-      simpl in H.
-      repeat rewrite HList.app_nil_r_trans in H.
-      eapply H in H0; clear H; auto. }
-  Qed.
-*)
